new/proof/github_com/google/btree_proof/btree_init.v
@@ -1,0 +1,15 @@
+From New.generatedproof.github_com.google Require Import btree.
+From New.proof Require Import proof_prelude.
+From New.proof Require Import fmt strings.
+From New.proof.sort_proof Require Import sort_init.
+From New.proof Require Import internal.race sync.atomic.
+From New.proof Require Import errors.
+
+Section proof.
+Context `{hG: heapGS Σ, !ffi_semantics _ _}.
+Context {sem : go.Semantics} {package_sem : btree.Assumptions}.
+Collection W := sem + package_sem.
+
+#[global] Instance : IsPkgInit (iProp Σ) btree := define_is_pkg_init True%I.
+#[global] Instance : GetIsPkgInitWf (iProp Σ) btree := build_get_is_pkg_init_wf.
+End proof.
