new/proof/github_com/google/btree_proof/query.v
@@ -1,0 +1,73 @@
+From New.generatedproof.github_com.google Require Import btree.
+From New.proof Require Import proof_prelude.
+From New.proof.github_com.google.btree_proof Require Import btree_init rep items.
+
+(** * Read-only btree operations: Get, Has, Len. *)
+
+Section proof.
+Context `{hG: heapGS Σ, !ffi_semantics _ _}.
+Context {sem : go.Semantics} {package_sem : btree.Assumptions}.
+Collection W := sem + package_sem.
+
+Set Default Proof Using "All".
+
+(** ** Len *)
+
+Lemma wp_BTree__Len R (t : loc) (elems : gset interface.t) :
+  {{{ is_pkg_init btree ∗ btree_repr R t elems }}}
+    #t @! (go.PointerType (btree.BTree)) @! "Len" #()
+  {{{ (n : w64), RET #n;
+      btree_repr R t elems ∗
+      ⌜uint.Z n = Z.of_nat (size elems)⌝ }}}.
+Proof. Admitted.
+
+(** ** node.get *)
+
+Lemma wp_node__get enforce_min height R
+    `{!RelDecision R, !Transitive R}
+    (n : loc) (elems : gset interface.t)
+    (degree : Z) (key : interface.t) :
+  {{{ is_pkg_init btree ∗
+      node_repr_aux enforce_min height R n elems degree ∗
+      is_less_fn R }}}
+    #n @! (go.PointerType (btree.node)) @! "get" #key
+  {{{ (result : interface.t) (found : bool), RET (#result, #found);
+      node_repr_aux enforce_min height R n elems degree ∗
+      ⌜if found then
+         result ∈ elems ∧ ¬R result key ∧ ¬R key result
+       else
+         ∀ e, e ∈ elems → R e key ∨ R key e⌝ }}}.
+Proof. Admitted.
+
+(** ** BTree.Get *)
+
+Lemma wp_BTree__Get R `{!RelDecision R, !Transitive R}
+    (t : loc) (elems : gset interface.t)
+    (key : interface.t) :
+  {{{ is_pkg_init btree ∗
+      btree_repr R t elems ∗
+      is_less_fn R }}}
+    #t @! (go.PointerType (btree.BTree)) @! "Get" #key
+  {{{ (result : interface.t) (found : bool), RET (#result, #found);
+      btree_repr R t elems ∗
+      ⌜if found then
+         result ∈ elems ∧ ¬R result key ∧ ¬R key result
+       else
+         ∀ e, e ∈ elems → R e key ∨ R key e⌝ }}}.
+Proof. Admitted.
+
+(** ** BTree.Has *)
+
+Lemma wp_BTree__Has R `{!RelDecision R, !Transitive R}
+    (t : loc) (elems : gset interface.t)
+    (key : interface.t) :
+  {{{ is_pkg_init btree ∗
+      btree_repr R t elems ∗
+      is_less_fn R }}}
+    #t @! (go.PointerType (btree.BTree)) @! "Has" #key
+  {{{ (b : bool), RET #b;
+      btree_repr R t elems ∗
+      ⌜b ↔ ∃ e, e ∈ elems ∧ ¬R e key ∧ ¬R key e⌝ }}}.
+Proof. Admitted.
+
+End proof.
